src/goose_lang/adequacy.v
@@ -49,6 +49,7 @@ Class gooseGpreS `{ext: ffi_syntax} `{EXT_SEM: !ffi_semantics ext ffi}
   #[global] goose_preG_ffi :: ffiGpreS Σ;
   #[global] goose_preG_trace :: trace_preG Σ;
   #[global] goose_preG_credit :: credit_preG Σ;
+  #[global] goose_preG_globals :: globals_preG Σ;
 }.
 
 Ltac solve_inG_deep :=
@@ -69,7 +70,7 @@ Ltac solve_inG_deep :=
                            end; intros; try done; split; assumption || by apply _.
 
 Definition heapΣ `{ext: ffi_syntax} `{ffi_interp_adequacy} : gFunctors :=
-  #[invΣ; crashΣ; na_heapΣ loc val; proph_mapΣ proph_id val; ffiΣ; traceΣ; creditΣ].
+  #[invΣ; crashΣ; na_heapΣ loc val; proph_mapΣ proph_id val; ffiΣ; traceΣ; creditΣ; globalsΣ].
 #[global]
 Instance subG_heapPreG `{ext: ffi_syntax} `{@ffi_interp_adequacy ffi Hinterp ext EXT} {Σ} :
   subG heapΣ Σ → gooseGpreS Σ.
