src/goose_lang/dist_lifting.v
@@ -15,6 +15,7 @@ Context `{@ffi_interp_adequacy ffi interp ext ffi_sem}.
 Definition wpd `{hG: !gooseGlobalGS Σ} (E: coPset) (ers: list node_init_cfg) :=
   ([∗ list] i↦σ ∈ ers, ∀ `(hG: !gooseLocalGS Σ),
     ffi_local_start (goose_ffiLocalGS) σ.(init_local_state).(world) -∗
+    own_globals (DfracOwn 1) σ.(init_local_state).(globals) -∗
     trace_frag σ.(init_local_state).(trace) -∗
     oracle_frag σ.(init_local_state).(oracle) ={E}=∗
     ∃ Φ Φrx Φinv, wpr NotStuck E σ.(init_thread) σ.(init_restart) Φ Φinv Φrx)%I.
